Add adequacy and chat server

chat_server.v
@@ -1,5 +1,189 @@
-From iris_io Require Import lang rules.
+From iris.proofmode Require Import tactics.
+From iris.program_logic Require Import weakestpre lifting.
+From iris_io Require Import lang rules petrinet channel.
 
 
+Section chat_server.
+  Context `{heapIG Σ, channelIG Σ, petrinetIG Σ}.
 
+  Variable ReceiveFromNick : iProp Σ → val → Stream val → iProp Σ.
+  Variable SendToNick : iProp Σ → val → Stream val → iProp Σ.
 
+  Definition token P : iProp Σ := P.
+
+  Variables send_to_nick receive_from_nick : expr.
+
+  Hypothesis send_to_nick_closed : ∀ f, send_to_nick.[f] = send_to_nick.
+  Hypothesis receive_from_nick_closed :
+    ∀ f, receive_from_nick.[f] = receive_from_nick.
+
+  Hint Rewrite send_to_nick_closed receive_from_nick_closed : autosubst.
+
+  Hypothesis wp_receive_from_nick : ∀ r n m μ,
+    {{{ token r ∗ ReceiveFromNick r n {| Shead := m; Stail := μ|} }}}
+      App receive_from_nick (of_val n)
+    {{{ RET m; ∃ r', token r' ∗ ReceiveFromNick r' n μ }}}.
+
+  Hypothesis wp_send_to_nick : ∀ s n m μ,
+    {{{ token s ∗ SendToNick s n {| Shead := m; Stail := μ|} }}}
+      App (App send_to_nick (of_val n)) (of_val m)
+    {{{ RET UnitV; ∃ s', token s' ∗ SendToNick s' n μ }}}.
+
+  Definition pumpFromNick :=
+    Lam
+      (Rec
+         (LetIn
+            (App receive_from_nick (Var 2))
+            (Seq
+               (App (App send (Var 2)) (Var 0))
+               (App (Var 1) (Var 2))
+            )
+         )
+      ).
+
+  Lemma pumpFromNick_closed f : pumpFromNick.[f] = pumpFromNick.
+  Proof. by asimpl. Qed.
+
+  Hint Rewrite pumpFromNick_closed : autosubst.
+
+  Lemma wp_pumpFromNick r roomCh n μ :
+    {{{ token r ∗ ReceiveFromNick r n μ ∗ sender roomCh μ }}}
+      App (App pumpFromNick (of_val n)) (of_val roomCh)
+    {{{RET UnitV; False}}}.
+  Proof.
+    iIntros (Φ) "(Hr & Hrfn & Hsnd) HΦ".
+    iApply (wp_bind (fill [AppLCtx _])).
+    iApply wp_pure_step_later; trivial.
+    iNext. asimpl.
+    iApply wp_value; simpl.
+    iLöb as "IH" forall (r μ).
+    iApply wp_pure_step_later; trivial.
+    iNext. asimpl.
+    iApply (wp_bind (fill [LetInCtx _])).
+    destruct μ as [m μ].
+    iApply (wp_receive_from_nick with "[$Hr $Hrfn]").
+    iNext. iDestruct 1 as (r') "[Hr' Hrfn]"; simpl.
+    iApply wp_pure_step_later; trivial.
+    iNext. asimpl.
+    iApply (wp_bind (fill [SeqCtx _])).
+    iApply (wp_send with "Hsnd").
+    iNext. iIntros "Hsnd"; simpl.
+    iApply wp_pure_step_later; trivial.
+    iNext. by iApply ("IH" with "Hr' Hrfn Hsnd").
+  Qed.
+
+  Typeclasses Opaque pumpFromNick.
+  Global Opaque pumpFromNick.
+
+  Definition pumpRoom :=
+    Lam (
+        Lam
+          (Rec(
+               LetIn
+                 (App receive (Var 1))
+                 (Seq
+                    (App (App send_to_nick (Var 4)) (Var 0))
+                    (Seq
+                       (App (App send_to_nick (Var 3)) (Var 0))
+                       (App (Var 1) (Var 2))
+                    )
+                 )
+             )
+          )
+      ).
+
+  Lemma pumpRoom_closed f : pumpRoom.[f] = pumpRoom.
+  Proof. by asimpl. Qed.
+
+  Hint Rewrite pumpRoom_closed : autosubst.
+
+  Lemma wp_pumpRoom roomCh s1 s2 n1 n2 μ :
+    {{{ token s1 ∗ SendToNick s1 n1 μ ∗ token s2 ∗ SendToNick s2 n2 μ
+              ∗ receiver roomCh μ }}}
+      App (App (App pumpRoom (of_val n1)) (of_val n2)) (of_val roomCh)
+    {{{RET UnitV; False}}}.
+  Proof.
+    iIntros (Φ) "(Hs1& Hn1 & Hs2 & Hn2 & Hrc) HΦ".
+    iApply (wp_bind (fill [AppLCtx _])).
+    iApply (wp_bind (fill [AppLCtx _])).
+    iApply wp_pure_step_later; trivial.
+    iNext. asimpl. iApply wp_value.
+    iApply wp_pure_step_later; trivial.
+    iNext. asimpl. iApply wp_value; simpl.
+    iLöb as "IH" forall (s1 s2 μ).
+    iApply wp_pure_step_later; trivial.
+    iNext. asimpl.
+    iApply (wp_bind (fill [LetInCtx _])).
+    destruct μ as [m μ].
+    iApply (wp_receive with "[$Hrc]").
+    iNext. iIntros "Hrc".
+    iApply wp_pure_step_later; trivial.
+    iNext. asimpl.
+    iApply (wp_bind (fill [SeqCtx _])).
+    iApply (wp_send_to_nick with "[$Hs1 $Hn1]").
+    iNext. iDestruct 1 as (s1') "[Hs1' Hn1]"; simpl.
+    iApply wp_pure_step_later; trivial.
+    iNext.
+    iApply (wp_bind (fill [SeqCtx _])).
+    iApply (wp_send_to_nick with "[$Hs2 $Hn2]").
+    iNext. iDestruct 1 as (s2') "[Hs2' Hn2]"; simpl.
+    iApply wp_pure_step_later; trivial.
+    iNext. by iApply ("IH" with "Hs1' Hn1 Hs2' Hn2 Hrc").
+  Qed.
+
+  Typeclasses Opaque pumpRoom.
+  Global Opaque pumpRoom.
+
+  Definition serveChatRoom n1 n2 :=
+    LetIn
+      (App new_channel Plang.Unit)
+      (Seq
+         (Fork (App (App pumpFromNick (of_val n1)) (Var 0)))
+         (Seq
+            (Fork (App (App pumpFromNick (of_val n2)) (Var 0)))
+            (App (App (App pumpRoom (of_val n1)) (of_val n2)) (Var 0))
+         )
+      ).
+
+  Definition SendToNicks s n1 n2 μ :=
+    (∃ s1 s2, (token s ==∗ token s1 ∗ token s2)
+                ∗ SendToNick s1 n1 μ ∗ SendToNick s2 n2 μ)%I.
+
+  Theorem wp_serverChatRoom n1 n2 r1 r2 s μ1 μ2 :
+    (∀ f, (of_val n1).[f] = (of_val n1)) →
+    (∀ f, (of_val n2).[f] = (of_val n2)) →
+    {{{ token r1 ∗ ReceiveFromNick r1 n1 μ1 ∗
+        token r2 ∗ ReceiveFromNick r2 n2 μ2 ∗
+        token s ∗ ∀ μ, ⌜interleaving μ1 μ2 μ⌝ → SendToNicks s n1 n2 μ }}}
+      serveChatRoom n1 n2
+  {{{RET UnitV; False}}}.
+  Proof.
+    iIntros (Hn1c Hn2c Φ) "(Hr1 & Hrc1 & Hr2 & Hrc2 & Hs & Hsnd) HΦ".
+    iApply (wp_bind (fill [LetInCtx _])).
+    iApply (wp_new_channel μ1 μ2); auto.
+    iNext; simpl.
+    iIntros (ch) "(Hsn1 & Hsn2 & Hsr)".
+    iDestruct "Hsr" as (μ) "[Hint Hrc]".
+    iDestruct "Hint" as %Hint.
+    iApply wp_pure_step_later; trivial.
+    iNext. asimpl; rewrite Hn1c Hn2c.
+    iApply (wp_bind (fill [SeqCtx _])).
+    iApply wp_fork; simpl; iSplitR "Hr1 Hrc1 Hsn1"; last first.
+    { by iApply (wp_pumpFromNick r1 with "[-]"); iFrame. }
+    iNext; iModIntro.
+    iApply wp_pure_step_later; trivial. iNext.
+    iApply (wp_bind (fill [SeqCtx _])).
+    iApply wp_fork; simpl; iSplitR "Hr2 Hrc2 Hsn2"; last first.
+    { by iApply (wp_pumpFromNick r2 with "[-]"); iFrame. }
+    iNext; iModIntro.
+    iApply wp_pure_step_later; trivial. iNext.
+    iDestruct ("Hsnd" $! μ Hint) as (s1 s2) "(Hsplit & Hsnd1 & Hsnd2)".
+    iMod ("Hsplit" with "Hs") as "[Hs1 Hs2]".
+    iApply (wp_pumpRoom _ s1 s2 with "[-HΦ]"); iFrame.
+  Qed.
+
+End chat_server.
+
+Hint Rewrite pumpFromNick_closed : autosubst.
+
+Hint Rewrite pumpRoom_closed : autosubst.
