adequacy.v
@@ -1,0 +1,52 @@
+From iris.program_logic Require Export weakestpre adequacy.
+From iris.program_logic Require Import ectx_lifting.
+From iris.base_logic Require Export invariants.
+From iris.algebra Require Import auth frac agree gmap.
+From iris_io Require Export lang rules proph_erasure full_erasure.
+From iris.proofmode Require Import tactics.
+From iris.base_logic Require Export gen_heap.
+
+Class heapIPreG Σ := HeapIPreG {
+  heapI_invG :> invPreG Σ;
+  heapI_gen_heapG :> gen_heapPreG loc val Σ;
+  prophI_gen_heapG :> gen_heapPreG loc (Stream val) Σ;
+  ioI_exclG :> inG Σ io_monoid;
+}.
+
+Definition IoΣ := #[invΣ; gen_heapΣ loc val; gen_heapΣ loc (Stream val);
+                      GFunctor io_monoid].
+
+Global Instance subG_io_monoid Σ : subG IoΣ Σ → inG Σ io_monoid.
+Proof. solve_inG. Qed.
+
+Theorem adequacy_instrumented Σ `{heapIPreG Σ} e Φ M :
+  (∀ `{Hig : heapIG Σ}, (WP e @ NotStuck; ⊤ {{ Φ }})%I) → safe e M.
+Proof.
+  intros Hwp.
+  cut (adequate NotStuck e {| Heap := ∅; Proph := ∅; ioState := M |} (λ _, True)).
+  { intros [Hrc Hns]; simpl in *.
+    intros th2 σ2 Hrtc e' He'.
+    specialize (Hns th2 σ2 e' eq_refl Hrtc He'); eauto. }
+  eapply wp_adequacy; first apply _.
+  iIntros (Hinv) "".
+  iMod (@own_alloc _ io_monoid _ (● Excl' (M : leibnizC ioSpec)))
+    as (γio) "HGI".
+  { split; last done. intros n; eapply ucmra_unit_leastN. }
+  iMod (gen_heap_init (∅ : gmap loc val)) as (Hheap) "Hheap".
+  iMod (gen_heap_init (∅ : gmap loc (Stream val))) as (Hproph) "Hproph".
+  set (HIG := {| γio := γio |} : heapIG Σ).
+  iModIntro.
+  iExists heapIG_stateI.
+  iSplitL; first by iFrame.
+    by (iApply wp_mono; last iApply Hwp; eauto).
+Qed.
+
+Theorem adequacy Σ `{heapIPreG Σ} (e : expr) Φ M :
+  prefix_closed M →
+  (∀ `{Hig : heapIG Σ}, (WP e @ NotStuck; ⊤ {{ Φ }})%I) → fully_erased_safe e M.
+Proof.
+  intros HPC Hig.
+  apply soundness_io; eauto.
+  apply soundness_prophecies.
+  eapply adequacy_instrumented; eauto.
+Qed.
